

Mathematical Background

Jan-2026

The Polynomial Remainder Theorem

We will develop the constructive proof briefly mentioned in the wikipedia article on [polynomial remainder theorem](#).

Let

$$f(x) = a_n x^n + a_{n-1} x^{n-1} + \dots + a_1 x + a_0$$

be a polynomial with coefficients in a ring, and let r be any element of the ring. Then there exists a polynomial $Q(x)$ of degree at most $(n-1)$ such that

$$f(x) = (x - r) Q(x) + f(r).$$

The remainder of the division of $f(x)$ by the linear polynomial $(x - r)$ is exactly $f(r)$.

Proof

The polynomial and its evaluation at r

Let

$$f(x) = a_n x^n + a_{n-1} x^{n-1} + \dots + a_1 x + a_0.$$

Evaluate $f(r)$:

$$f(r) = a_n r^n + a_{n-1} r^{n-1} + \dots + a_1 r + a_0.$$

The difference $f(x) - f(r)$

$$\begin{aligned} f(x) - f(r) &= (a_n x^n + a_{n-1} x^{n-1} + \dots + a_1 x + a_0) - (a_n r^n + a_{n-1} r^{n-1} + \dots + a_1 r + a_0). \\ &= (a_n x^n - a_n r^n) + (a_{n-1} x^{n-1} - a_{n-1} r^{n-1}) + \dots + (a_1 x - a_1 r) + (a_0 - a_0) \\ &= \underbrace{a_n(x^n - r^n)}_{\text{TERM } n} + \underbrace{a_{n-1}(x^{n-1} - r^{n-1})}_{\text{TERM } n-1} + \dots + \underbrace{a_1(x - r)}_{\text{TERM } 1} \end{aligned}$$

Recall the algebraic identity

$$\begin{aligned} x^k - r^k &= (x - r)(x^{k-1} + x^{k-2}r + \dots + xr^{k-2} + r^{k-1}) \quad \text{for an integer } k \geq 1. \\ a_k(x^k - r^k) &= a_k(x - r)(x^{k-1} + x^{k-2}r + \dots + xr^{k-2} + r^{k-1}) \quad \text{for } k = 1, \dots, n. \end{aligned}$$

Apply the identity to each term in $f(x) - f(r)$

Consider the term $a_n(x^n - r^n)$ in the above equation, and substitute

$$a_k(x^k - r^k) = (x - r) a_k(x^{k-1} + x^{k-2}r + \dots + r^{k-1}) \quad 1 \leq k \leq n.$$

Rewriting the terms in (5) gives

$$\begin{aligned} a_n(x^n - r^n) &= (x - r) a_n(x^{n-1} + x^{n-2}r + \dots + r^{n-1}) \\ a_n(x^{n-1} - r^{n-1}) &= (x - r) a_{n-1}(x^{n-2} + x^{n-3}r + \dots + r^{n-2}) \\ &\vdots \\ a_1(x - r) &= (x - r) a_1 \end{aligned}$$

Factor out $(x - r)$.

$$\begin{aligned} f(x) - f(r) &= (x - r) a_n(x^{n-1} + x^{n-2}r + \dots + r^{n-1}) \\ &\quad + (x - r) a_{n-1}(x^{n-2} + x^{n-3}r + \dots + r^{n-2}) \\ &\quad + \dots + (x - r) a_1. \end{aligned}$$

Factor $(x - r)$ from the entire sum (the right-hand side expression):

$$f(x) - f(r) = (x - r) \left(a_n(x^{n-1} + x^{n-2}r + \dots + r^{n-1}) + \dots + a_1 \right).$$

Define the polynomial $Q(x)$ and Complete the Proof

Let

$$Q(x) = a_n(x^{n-1} + x^{n-2}r + \dots + r^{n-1}) + a_{n-1}(x^{n-2} + x^{n-3}r + \dots + r^{n-2}) + \dots + a_1.$$

where

$$\deg(Q) \leq n - 1$$

We use polynomial Q , and write

$$f(x) - f(r) = (x - r) Q(x).$$

from which it follows that

$$f(x) = (x - r) Q(x) + f(r).$$

■